src/program_proof/tulip/res_group.v
@@ -1,4 +1,5 @@
-(** Global resources. *)
+From iris.algebra Require Import mono_nat mono_list gmap_view gset.
+From iris.algebra.lib Require Import dfrac_agree.
 From Perennial.program_proof Require Import grove_prelude.
 From Perennial.program_proof.tulip Require Import base.
 
@@ -12,16 +13,20 @@ Section res.
 
     (** Mapping from transaction IDs to preparedness of transactions on a group. *)
 
-    Definition own_group_prepm γ (gid : u64) (pm : gmap nat bool) : iProp Σ.
-    Admitted.
+    Definition is_group_prep γ (gid : u64) (ts : nat) (p : bool) : iProp Σ :=
+      own γ.(group_prep) {[ gid := gmap_view_frag ts DfracDiscarded (to_agree p) ]}.
 
-    Definition is_group_prep γ (gid : u64) (ts : nat) (p : bool) : iProp Σ.
-    Admitted.
+    Definition own_group_prepm_auth γ (gid : u64) (pm : gmap nat bool) : iProp Σ :=
+      own γ.(group_prep) {[ gid := gmap_view_auth (DfracOwn 1) (to_agree <$> pm) ]}.
+
+    Definition own_group_prepm γ (gid : u64) (pm : gmap nat bool) : iProp Σ :=
+      own_group_prepm_auth γ gid pm ∗
+      ([∗ map] ts ↦ p ∈ pm, is_group_prep γ gid ts p).
 
     #[global]
     Instance is_group_prep_persistent γ gid ts p :
       Persistent (is_group_prep γ gid ts p).
-    Admitted.
+    Proof. apply _. Defined.
 
     Definition is_group_prepared γ gid ts :=
       is_group_prep γ gid ts true.
@@ -33,25 +38,57 @@ Section res.
       is_group_prep γ gid ts p1 -∗
       is_group_prep γ gid ts p2 -∗
       ⌜p2 = p1⌝.
-    Admitted.
+    Proof.
+      iIntros "Hfrag1 Hfrag2".
+      iDestruct (own_valid_2 with "Hfrag1 Hfrag2") as %Hvalid.
+      rewrite singleton_op singleton_valid in Hvalid.
+      apply gmap_view_frag_op_valid in Hvalid as [_ Hvalid].
+      by apply to_agree_op_inv_L in Hvalid.
+    Qed.
 
     Lemma group_prep_insert {γ gid pm} ts p :
       pm !! ts = None ->
       own_group_prepm γ gid pm ==∗
       own_group_prepm γ gid (<[ts := p]> pm) ∗ is_group_prep γ gid ts p.
-    Admitted.
+    Proof.
+      iIntros (Hnotin) "[Hauth #Hfrags]".
+      iAssert (own_group_prepm_auth γ gid (<[ts := p]> pm) ∗ is_group_prep γ gid ts p)%I
+        with "[> Hauth]" as "[Hauth #Hfrag]".
+      { iRevert "Hauth".
+        rewrite -own_op.
+        iApply own_update.
+        rewrite singleton_op.
+        apply singleton_update.
+        rewrite fmap_insert. apply: gmap_view_alloc; [|done..].
+        by rewrite lookup_fmap Hnotin.
+      }
+      iFrame "∗ #".
+      by iApply big_sepM_insert_2.
+    Qed.
 
     Lemma group_prep_lookup γ gid pm ts p :
       own_group_prepm γ gid pm -∗
       is_group_prep γ gid ts p -∗
       ⌜pm !! ts = Some p⌝.
-    Admitted.
+    Proof.
+      iIntros "[Hauth _] Hfrag".
+      iDestruct (own_valid_2 with "Hauth Hfrag") as %Hvalid.
+      rewrite singleton_op singleton_valid in Hvalid.
+      apply gmap_view_both_dfrac_valid_discrete_total in Hvalid.
+      destruct Hvalid as (v' & _ & _ & Hlookup & _ & Hincl).
+      apply lookup_fmap_Some in Hlookup as (b & <- & Hb).
+      apply to_agree_included_L in Hincl.
+      by subst b.
+    Qed.
 
     Lemma group_prep_witness γ gid pm ts p :
       pm !! ts = Some p ->
       own_group_prepm γ gid pm -∗
       is_group_prep γ gid ts p.
-    Admitted.
+    Proof.
+      iIntros (Hp) "[_ Hfrags]".
+      by iApply (big_sepM_lookup with "Hfrags").
+    Qed.
 
   End group_prep.
 
@@ -59,23 +96,58 @@ Section res.
 
     (** Mapping from transaction IDs to proposals (i.e., pairs of rank and bool). *)
 
-    Definition own_group_prepare_proposals_map
-      γ (gid : u64) (psm : gmap nat (gmap nat bool)) : iProp Σ.
-    Admitted.
+    Definition is_group_prepare_proposal γ (gid : u64) (ts : nat) (rk : nat) (p : bool) : iProp Σ :=
+      own γ.(group_prepare_proposal)
+              {[ gid := (gmap_view_frag (ts, rk) DfracDiscarded (to_agree p)) ]}.
 
-    Definition is_group_prepare_proposal γ (gid : u64) (ts : nat) (rk : nat) (p : bool) : iProp Σ.
-    Admitted.
+    Definition own_group_ppsl_auth γ (gid : u64) (psm : gmap (nat * nat) bool) : iProp Σ :=
+      own γ.(group_prepare_proposal) {[ gid := (gmap_view_auth (DfracOwn 1) (to_agree <$> psm)) ]}.
+
+    Definition own_group_prepare_proposals_map
+      γ (gid : u64) (psm : gmap nat (gmap nat bool)) : iProp Σ :=
+      ∃ m : gmap (nat * nat) bool,
+        own_group_ppsl_auth γ gid m ∗
+        ([∗ map] tr ↦ p ∈ m, is_group_prepare_proposal γ gid tr.1 tr.2 p) ∗
+        (⌜∀ t r p, m !! (t, r) = Some p ↔ ∃ im, psm !! t = Some im ∧ im !! r = Some p⌝).
 
     #[global]
     Instance is_group_prepare_proposal_persistent γ gid ts rk p :
       Persistent (is_group_prepare_proposal γ gid ts rk p).
-    Admitted.
+    Proof. apply _. Defined.
 
-    Lemma group_prepare_proposal_init {γ gid psm} ts ps :
+    (* TODO: this doesn't need an update modality *)
+    Lemma group_prepare_proposal_init {γ gid psm} ts :
       psm !! ts = None ->
       own_group_prepare_proposals_map γ gid psm ==∗
-      own_group_prepare_proposals_map γ gid (<[ts := ps]> psm).
-    Admitted.
+      own_group_prepare_proposals_map γ gid (<[ts := ∅]> psm).
+    Proof.
+      iIntros (Hnotin) "Hauth".
+      iDestruct "Hauth" as (m) "(Hauth & Hppsl & %Heq)".
+      iExists m.
+      iFrame.
+      iPureIntro.
+      intros t r p.
+      split.
+      { intros Hp.
+        specialize (Heq t r p).
+        destruct Heq as [Hincl _].
+        specialize (Hincl Hp).
+        destruct Hincl as (im & Him & Himr).
+        destruct (decide (t = ts)) as [-> | Hne]; first congruence.
+        exists im.
+        by rewrite lookup_insert_ne.
+      }
+      { intros (im & Him & Hp).
+        specialize (Heq t r p).
+        destruct Heq as [_ Hincl].
+        apply Hincl.
+        destruct (decide (ts = t)) as [-> | Hne].
+        { rewrite lookup_insert in Him. inv Him. }
+        { rewrite lookup_insert_ne in Him; last done.
+          by eauto.
+        }
+      }
+    Qed.
 
     Lemma group_prepare_proposal_insert {γ gid psm} ts ps rk p :
       let ps' := <[rk := p]> ps in
@@ -83,20 +155,114 @@ Section res.
       ps !! rk = None ->
       own_group_prepare_proposals_map γ gid psm ==∗
       own_group_prepare_proposals_map γ gid (<[ts := ps']> psm).
-    Admitted.
+    Proof.
+      iIntros (ps' Hps Hnotin) "Hauth".
+      iDestruct "Hauth" as (m) "(Hauth & Hppsl & %Heq)".
+      iAssert (own_group_ppsl_auth γ gid (<[(ts, rk) := p]> m) ∗
+               is_group_prepare_proposal γ gid ts rk p)%I
+        with "[> Hauth]" as "[Hauth #Hfrag]".
+      { iRevert "Hauth".
+        rewrite -own_op.
+        iApply own_update.
+        rewrite singleton_op.
+        apply singleton_update.
+        rewrite fmap_insert. apply: gmap_view_alloc; [|done..].
+        rewrite lookup_fmap.
+        destruct (m !! (ts, rk)) as [p' |] eqn:Hin; last done.
+        specialize (Heq ts rk p').
+        destruct Heq as [Hincl _].
+        specialize (Hincl Hin).
+        destruct Hincl as (im & Him & Hp').
+        rewrite Hps in Him. inv Him.
+      }
+      iExists (<[(ts, rk) := p]> m).
+      iFrame.
+      iModIntro.
+      iSplit.
+      { by iApply big_sepM_insert_2. }
+      iPureIntro.
+      intros t r p'.
+      split.
+      { intros Hp'.
+        destruct (decide (t = ts)) as [-> | Hne].
+        { rewrite lookup_insert.
+          exists ps'.
+          split; first done.
+          subst ps'.
+          destruct (decide (r = rk)) as [-> | Hner].
+          { rewrite lookup_insert.
+            by rewrite lookup_insert in Hp'.
+          }
+          { rewrite lookup_insert_ne; last done.
+            rewrite lookup_insert_ne in Hp'; last first.
+            { intros Hcontra. inv Hcontra. }
+            specialize (Heq ts r p').
+            destruct Heq as [Hincl _].
+            specialize (Hincl Hp').
+            destruct Hincl as (im & Him & Himr).
+            rewrite Hps in Him. by inv Him.
+          }
+        }
+        { rewrite lookup_insert_ne; last done.
+          rewrite lookup_insert_ne in Hp'; last first.
+          { intros Hcontra. inv Hcontra. }
+          by apply Heq.
+        }
+      }
+      { intros Him.
+        destruct Him as (im & Him & Hp').
+        destruct (decide (t = ts)) as [-> | Hne].
+        { rewrite lookup_insert in Him. inv Him.
+          destruct (decide (r = rk)) as [-> | Hner].
+          { rewrite lookup_insert.
+            rewrite lookup_insert in Hp'. by inv Hp'.
+          }
+          { rewrite lookup_insert_ne; last first.
+            { intros Hcontra. inv Hcontra. }
+            rewrite lookup_insert_ne in Hp'; last done.
+            apply Heq.
+            by eauto.
+          }
+        }
+        { rewrite lookup_insert_ne; last first.
+          { intros Hcontra. inv Hcontra. }
+          rewrite lookup_insert_ne in Him; last done.
+          apply Heq.
+          by eauto.
+        }
+      }
+    Qed.
 
     Lemma group_prepare_proposal_witness {γ gid psm} ts ps rk p :
       psm !! ts = Some ps ->
       ps !! rk = Some p ->
       own_group_prepare_proposals_map γ gid psm -∗
       is_group_prepare_proposal γ gid ts rk p.
-    Admitted.
+    Proof.
+      iIntros (Hps Hp) "Hauth".
+      iDestruct "Hauth" as (im) "(_ & Hfrags & %Heq)".
+      iApply (big_sepM_lookup _ _ (ts, rk) with "Hfrags").
+      apply Heq.
+      by eauto.
+    Qed.
 
     Lemma group_prepare_proposal_lookup γ gid psm ts rk p :
       is_group_prepare_proposal γ gid ts rk p -∗
       own_group_prepare_proposals_map γ gid psm -∗
       ∃ ps, ⌜psm !! ts = Some ps ∧ ps !! rk = Some p⌝.
-    Admitted.
+    Proof.
+      iIntros "Hfrag Hauth".
+      iDestruct "Hauth" as (im) "(Hauth & _ & %Heq)".
+      iDestruct (own_valid_2 with "Hauth Hfrag") as %Hvalid.
+      rewrite singleton_op singleton_valid in Hvalid.
+      apply gmap_view_both_dfrac_valid_discrete_total in Hvalid.
+      destruct Hvalid as (v' & _ & _ & Hlookup & _ & Hincl).
+      apply lookup_fmap_Some in Hlookup as (b & <- & Hb).
+      apply to_agree_included_L in Hincl.
+      subst b.
+      iPureIntro.
+      by apply Heq.
+    Qed.
 
   End group_prepare_proposal.
 
@@ -104,16 +270,20 @@ Section res.
 
     (** Mapping from transaction IDs to committedness of transactions on a group. *)
 
-    Definition own_group_commit_map γ (gid : u64) (pm : gmap nat bool) : iProp Σ.
-    Admitted.
+    Definition is_group_commit γ (gid : u64) (ts : nat) (c : bool) : iProp Σ :=
+      own γ.(group_commit) {[ gid := (gmap_view_frag ts DfracDiscarded (to_agree c)) ]}.
 
-    Definition is_group_commit γ (gid : u64) (ts : nat) (c : bool) : iProp Σ.
-    Admitted.
+    Definition own_group_commit_map_auth γ (gid : u64) (cm : gmap nat bool) : iProp Σ :=
+      own γ.(group_commit) {[ gid := (gmap_view_auth (DfracOwn 1) (to_agree <$> cm)) ]}.
+
+    Definition own_group_commit_map γ (gid : u64) (cm : gmap nat bool) : iProp Σ :=
+      own_group_commit_map_auth γ gid cm ∗
+      ([∗ map] ts ↦ c ∈ cm, is_group_commit γ gid ts c).
 
     #[global]
     Instance is_group_commit_persistent γ gid ts c :
       Persistent (is_group_commit γ gid ts c).
-    Admitted.
+    Proof. apply _. Defined.
 
     Definition is_group_committed γ gid ts :=
       is_group_commit γ gid ts true.
@@ -125,25 +295,57 @@ Section res.
       is_group_commit γ gid ts c1 -∗
       is_group_commit γ gid ts c2 -∗
       ⌜c2 = c1⌝.
-    Admitted.
+    Proof.
+      iIntros "Hfrag1 Hfrag2".
+      iDestruct (own_valid_2 with "Hfrag1 Hfrag2") as %Hvalid.
+      rewrite singleton_op singleton_valid in Hvalid.
+      apply gmap_view_frag_op_valid in Hvalid as [_ Hvalid].
+      by apply to_agree_op_inv_L in Hvalid.
+    Qed.
 
     Lemma group_commit_insert {γ gid pm} ts c :
       pm !! ts = None ->
       own_group_commit_map γ gid pm ==∗
       own_group_commit_map γ gid (<[ts := c]> pm) ∗ is_group_commit γ gid ts c.
-    Admitted.
+    Proof.
+      iIntros (Hnotin) "[Hauth #Hfrags]".
+      iAssert (own_group_commit_map_auth γ gid (<[ts := c]> pm) ∗ is_group_commit γ gid ts c)%I
+        with "[> Hauth]" as "[Hauth #Hfrag]".
+      { iRevert "Hauth".
+        rewrite -own_op.
+        iApply own_update.
+        rewrite singleton_op.
+        apply singleton_update.
+        rewrite fmap_insert. apply: gmap_view_alloc; [|done..].
+        by rewrite lookup_fmap Hnotin.
+      }
+      iFrame "∗ #".
+      by iApply big_sepM_insert_2.
+    Qed.
 
     Lemma group_commit_witness γ gid pm ts c :
       pm !! ts = Some c ->
       own_group_commit_map γ gid pm -∗
       is_group_commit γ gid ts c.
-    Admitted.
+    Proof.
+      iIntros (Hp) "[_ Hfrags]".
+      by iApply (big_sepM_lookup with "Hfrags").
+    Qed.
 
     Lemma group_commit_lookup γ gid pm ts c :
       own_group_commit_map γ gid pm -∗
       is_group_commit γ gid ts c -∗
       ⌜pm !! ts = Some c⌝.
-    Admitted.
+    Proof.
+      iIntros "[Hauth _] Hfrag".
+      iDestruct (own_valid_2 with "Hauth Hfrag") as %Hvalid.
+      rewrite singleton_op singleton_valid in Hvalid.
+      apply gmap_view_both_dfrac_valid_discrete_total in Hvalid.
+      destruct Hvalid as (v' & _ & _ & Hlookup & _ & Hincl).
+      apply lookup_fmap_Some in Hlookup as (b & <- & Hb).
+      apply to_agree_included_L in Hincl.
+      by subst b.
+    Qed.
 
   End group_commit.
 
